crates/correctness/lean/MxxCorrectness/Generated/ToyExample/Ir.lean
@@ -12,7 +12,7 @@ def ToyExample_protocolSourceHash : String := "c894ed871c835c66f3dbb1c42a53b03a5
 
 def ToyExample_workflowHash : String := "f0727b300c312d49e01c5cba55cf8d11de69de7efa5d17b68a4133c5a6a15c6b"
 
-def ToyExample_toolkitHash : String := "f37fe0a1116ae90d8d896b635a03a982ba04d9aa7f6efe3af03d6eb82234cd7d"
+def ToyExample_toolkitHash : String := "944154b5aebd28b16b744fc734d61ea0f4d5913a5ab94aaaf74df85b34a0a4d5"
 
 def ToyExample_derivationHash : String := "1eb7ee1d85bf85dc59fea9e4e198e1cfa94df8fd0bf8168d408a754514520933"
 
